src/cbor/pulse/CBOR.Pulse.API.Det.Rust.fsti
@@ -38,32 +38,7 @@ val cbor_det_size
       pure (cbor_det_size_postcond y bound res)
     )
 
-noextract [@@noextract_to "krml"]
-let cbor_det_serialize_postcond
-  (y: Spec.cbor)
-  (v: Seq.seq U8.t)
-  (v': Seq.seq U8.t)
-  (res: option SZ.t)
-: Tot prop
-= let s = Spec.cbor_det_serialize y in
-  match res with
-  | None -> Seq.length s > Seq.length v /\ v' == v
-  | Some len ->
-    Seq.length s == SZ.v len /\
-    SZ.v len <= Seq.length v /\
-    v' `Seq.equal` (s `Seq.append` Seq.slice v (SZ.v len) (Seq.length v))
-
-val cbor_det_serialize
-  (x: cbordet)
-  (output: S.slice U8.t)
-  (#y: Ghost.erased Spec.cbor)
-  (#pm: perm)
-  (#v: Ghost.erased (Seq.seq U8.t))
-: stt (option SZ.t)
-    (cbor_det_match pm x y ** pts_to output v)
-    (fun res -> exists* v' . cbor_det_match pm x y ** pts_to output v' ** pure (
-      cbor_det_serialize_postcond y v v' res
-    ))
+val cbor_det_serialize (_: unit) : Base.cbor_det_serialize_t cbor_det_match
 
 (* Constructors *)
 
